work

tests/elab/symm.lean
@@ -1,14 +1,72 @@
 import Init.Tactics
 
+/-!
+# Tests of the @[symm] attribute and `symm` tactic
+
+See also `tests/elab/relationAttrs.lean`
+-/
+
 set_option autoImplicit true
 set_option linter.missingDocs false
+-- For testing:
+--set_option trace.Meta.Tactic.relation true
 
--- testing that the attribute is recognized
-@[symm] def eq_symm {α : Type} (a b : α) : a = b → b = a := Eq.symm
+/-! Basic tests of symmetry for `Eq`. -/
+/--
+trace: a b : Nat
+a✝ : a = b
+⊢ a = b
+-/
+#guard_msgs in
+example (a b : Nat) : a = b → b = a := by intros; symm; trace_state; assumption
+/--
+trace: a b : Nat
+h : b = a
+a✝ : True
+⊢ b = a
+-/
+#guard_msgs in
+example (a b : Nat) : a = b → True → b = a := by intro h _; symm at h; trace_state; assumption
 
-example (a b : Nat) : a = b → b = a := by intros; symm; assumption
-example (a b : Nat) : a = b → True → b = a := by intro h _; symm at h; assumption
+/-! Basic tests of symmetry for `Iff`. -/
+/--
+trace: a b : Prop
+a✝ : a ↔ b
+⊢ a ↔ b
+-/
+#guard_msgs in
+example (a b : Prop) : (a ↔ b) → (b ↔ a) := by intros; symm; trace_state; assumption
+/--
+trace: a b : Prop
+h : b ↔ a
+a✝ : True
+⊢ b ↔ a
+-/
+#guard_msgs in
+example (a b : Prop) : (a ↔ b) → True → (b ↔ a) := by intro h _; symm at h; trace_state; assumption
 
+/-! Basic tests of symmetry for `Eq`. -/
+/--
+trace: α β : Type u
+a : α
+b : β
+a✝ : a ≍ b
+⊢ a ≍ b
+-/
+#guard_msgs in
+example {α β : Type u} (a : α) (b : β) : a ≍ b → b ≍ a := by intros; symm; trace_state; assumption
+/--
+trace: α β : Type u
+a : α
+b : β
+h : b ≍ a
+a✝ : True
+⊢ b ≍ a
+-/
+#guard_msgs in
+example {α β : Type u} (a : α) (b : β) : a ≍ b → True → b ≍ a := by intro h _; symm at h; trace_state; assumption
+
+/-! Basic tests with a custom relation. -/
 def sameParity : Nat → Nat → Prop
   | n, m => n % 2 = m % 2
 
@@ -16,12 +74,87 @@ def sameParity : Nat → Nat → Prop
 
 example (a b : Nat) : sameParity a b → sameParity b a := by intros; symm; assumption
 
+/-! Basic tests with a custom relation. -/
 def MyEq (n m : Nat) := ∃ k, n + k = m ∧ m + k = n
 
 @[symm] theorem MyEq.symm {n m : Nat} (h : MyEq n m) : MyEq m n := by
   rcases h with ⟨k, h1, h2⟩
   exact ⟨k, h2, h1⟩
 
+/--
+trace: n m : Nat
+h : MyEq n m
+⊢ MyEq n m
+-/
+#guard_msgs in
 example {n m : Nat} (h : MyEq n m) : MyEq m n := by
   symm
+  trace_state
   assumption
+
+/--
+trace: n m : Nat
+h : MyEq m n
+⊢ MyEq m n
+-/
+#guard_msgs in
+example {n m : Nat} (h : MyEq n m) : MyEq m n := by
+  symm at h
+  trace_state
+  assumption
+
+/-! Contraposition -/
+/--
+trace: n m : Nat
+h : ¬MyEq n m
+⊢ ¬MyEq n m
+-/
+#guard_msgs in
+theorem MyEq.nsymm {n m : Nat} (h : ¬ MyEq n m) : ¬ MyEq m n := by
+  symm
+  trace_state
+  exact h
+
+/-- info: 'MyEq.nsymm' does not depend on any axioms -/
+#guard_msgs in #print axioms MyEq.nsymm
+
+/-! Contraposition at a local hypothesis -/
+/--
+trace: n m : Nat
+h : ¬MyEq m n
+⊢ ¬MyEq m n
+-/
+#guard_msgs in
+theorem MyEq.nsymm' {n m : Nat} (h : ¬ MyEq n m) : ¬ MyEq m n := by
+  symm at h
+  trace_state
+  exact h
+
+/-- info: 'MyEq.nsymm'' does not depend on any axioms -/
+#guard_msgs in #print axioms MyEq.nsymm'
+
+
+/-! Unfolding abbreviations -/
+abbrev MyNEq (n m : Nat) := ¬ MyEq m n
+
+/--
+trace: n m : Nat
+h : MyNEq n m
+⊢ ¬MyEq m n
+-/
+#guard_msgs in
+example {n m : Nat} (h : MyNEq n m) : MyNEq m n := by
+  symm
+  trace_state
+  exact h
+
+/--
+trace: n m : Nat
+h : ¬MyEq n m
+⊢ MyNEq m n
+-/
+#guard_msgs in
+example {n m : Nat} (h : MyNEq n m) : MyNEq m n := by
+  symm at h
+  trace_state
+  exact h
