src/Lean/Meta/Tactic/Symm.lean
@@ -10,6 +10,8 @@ public import Lean.Meta.Tactic.Assert
 public import Lean.Meta.DiscrTree.Main
 import Lean.Meta.AppBuilder
 import Lean.Meta.Tactic.Apply
+import Lean.Meta.Tactic.Clear
+import Lean.Meta.Tactic.Relations
 import Lean.Elab.Tactic.Basic
 public section
 
@@ -20,7 +22,7 @@ This implements the `symm` tactic, which can apply symmetry theorems to either t
 hypothesis.
 -/
 
-open Lean Meta
+open Lean Meta Elab
 
 namespace Lean.Meta.Symm
 
@@ -32,11 +34,9 @@ builtin_initialize symmExt :
     initial := {}
   }
 
-/-- Returns the symmetry lemmas that match the target type. -/
-def getSymmLemmas (tgt : Expr) : MetaM (Expr × Array Name) := do
-  let .app (.app rel _) _ := tgt
-    | throwError "Symmetry lemmas only apply to binary relations, not{indentExpr tgt}"
-  return (rel, ← (symmExt.getState (← getEnv)).getMatch rel)
+/-- Returns the symmetry lemmas that match the given relation. -/
+def getSymmLemmas (rel : Expr) : MetaM (Array Name) := do
+  (symmExt.getState (← getEnv)).getMatch rel
 
 /--
 Tags symmetry lemmas to be used by the `symm` tactic.
@@ -48,50 +48,218 @@ builtin_initialize registerBuiltinAttribute {
   name := `symm
   descr := "symmetric relation"
   add := fun decl _ kind => MetaM.run' do
-    let declTy ← inferType (← mkConstWithFreshMVarLevels decl)
-    let (_, _, targetTy) ← withReducible <| forallMetaTelescopeReducing declTy
-    let fail := throwError
-      "@[symm] attribute only applies to lemmas proving x ∼ y → y ∼ x, got {declTy}"
-    -- Note: this checks that `targetTy` has at least two arguments.
-    -- There's no guarantee that the last two arguments are the arguments to the relation!
-    -- Possibly there are instance arguments after the main arguments. This is an approximation.
-    let .app (.app rel _) _ ← whnfR targetTy | fail
-    -- Instantiate another copy, then try unifying its last argument with the target.
-    let declTy' ← inferType (← mkConstWithFreshMVarLevels decl)
-    let (xs', _, _) ← withReducible <| forallMetaTelescopeReducing declTy'
-    let some h := xs'.back? | fail
-    unless ← withoutModifyingMCtx (do isDefEq targetTy (← inferType h)) do fail
-    let key ← DiscrTree.mkPath rel
-    symmExt.add (decl, key) kind
+    withTraceNode `Meta.Tactic.relation (fun _ => return m!"adding [symm] lemma `{.ofConstName decl}`") do
+      let declTy := (← getConstInfo decl).type
+      forallTelescope declTy fun xs targetTy => do
+        let targetTy ← whnfCore targetTy
+        let .const relName _ := targetTy.getAppFn
+          | throwError "\
+              `[symm]` attribute only applies to lemmas proving `x ∼ y → y ~ x`, where the relation is \
+              a constant application, but the relation is not a constant application:\
+              {inlineExprTrailing targetTy}"
+        -- If the this isn't a registered relation, automatically infer and register it.
+        if (← getRelationInfo? relName).isNone then
+          withTraceNode `Meta.Tactic.relation (fun _ => return m!"Unknown relation, inferring [relation] for `{.ofConstName relName}`.") do
+            let info ← inferRelationInfo relName #[]
+            registerRelation relName info kind
+        let some info ← matchesRelation? targetTy | unreachable!
+        -- Validate last argument of the lemma
+        if xs.isEmpty then
+          throwError "`[symm]` attribute only applies to lemmas proving `x ~ y → y ~ x`, but the `{.ofConstName decl}` has no hypotheses"
+        let hypTy ← whnfCore (← xs.back!.fvarId!.getType)
+        unless hypTy.getAppFn.constName? == relName do
+          throwError "`[symm]` attribute only applies to lemmas proving `x ~ y → y ~ x`, but the last hypothesis `{.ofConstName decl}` is not an application of the conclusion's relation{inlineExprTrailing info.rel}"
+        let some hypInfo ← matchesRelation? hypTy | panic! "`[symm]` unexpectedly could not analyze hypothesis relation"
+        -- Validate that symmetry is being applied
+        unless ← isDefEq info.lhs hypInfo.rhs do
+          let (lhs, hypRhs) ← addPPExplicitToExposeDiff info.lhs hypInfo.rhs
+          throwError "\
+            `[symm]` attribute only applies to lemmas proving `x ~ y → y ∼ x`, \
+            but the conclusion's left-hand side{indentExpr lhs}\nis not definitionally equal to the hypothesis's right-hand side{indentExpr hypRhs}"
+        unless ← isDefEq info.rhs hypInfo.lhs do
+          let (rhs, hypLhs) ← addPPExplicitToExposeDiff info.rhs hypInfo.lhs
+          throwError "\
+            `[symm]` attribute only applies to lemmas proving `x ~ y → y ∼ x`, \
+            but the conclusion's right-hand side{indentExpr rhs}\nis not definitionally equal to the hypothesis's left-hand side{indentExpr hypLhs}"
+        -- Validate applicability of the lemma
+        let g ← mkFreshExprSyntheticOpaqueMVar targetTy
+        let gs ← g.mvarId!.apply (← mkConstWithFreshMVarLevels decl) (term? := m!"'{.ofConstName decl}'")
+        unless gs.length == 1 do
+          let gs ← gs.filterM fun g => not <$> withNewMCtxDepth do isDefEq (← g.getType) hypTy
+          throwError "`[symm]` lemma has unsolved goals when applied to its own conclusion\n{goalsToMessageData gs}"
+      let (_, _, targetTy) ← forallMetaTelescope declTy
+      let some info ← matchesRelation? (← whnfCore targetTy) | unreachable!
+      let key ← DiscrTree.mkPath info.rel
+      symmExt.add (decl, key) kind
 }
 
-def forEachSymmLemma {α} (g? : Option MVarId) (tgt : Expr)
-    (k : Expr → Expr → Array Expr → Expr → Expr → MetaM α) : MetaM α := do
-  let tgt ← instantiateMVars (← whnfR tgt)
-  let (rel, lems) ← getSymmLemmas tgt
-  let s ← saveState
-  let mut ex? := none
-  for lem in lems do
-    try
-      let lem ← mkConstWithFreshMVarLevels lem
-      let (args, bis, body) ← withReducible <| forallMetaTelescopeReducing (← inferType lem)
-      let some eArg := args.back? | panic! "invalid symm lemma"
-      let res ← k lem tgt args body eArg
-      synthAppInstances `symm g? args.pop bis.pop (allowSynthFailures := false) (synthAssignedInstances := true)
-      let gs ← args.pop.filterM fun arg => not <$> arg.mvarId!.isAssigned
-      unless gs.isEmpty do
-        throwError MessageData.tagged `Tactic.unsolvedGoals <| m!"unsolved goals\n{Elab.goalsToMessageData (gs.map Expr.mvarId!).toList}"
-      return res
-    catch e =>
-      unless ex?.isSome do
-        ex? := some (← saveState, e)
-    s.restore
-  if let some (sErr, e) := ex? then
-    sErr.restore
-    throw e
+private def noSymmLemmaMsg (rel : Expr) : MessageData :=
+  m!"No `[symm]` lemma registered for relation{indentExpr rel}"
+    ++ MessageData.hint' m!"Add the `[sym]` attribute to symmetry lemmas for{inlineExpr rel}to use this tactic"
+
+private def throwNoSymmLemma {α} (goal? : Option MVarId) (rel : Expr) : MetaM α :=
+  throwTacticEx `symm goal? <| noSymmLemmaMsg rel
+
+private def throwRelError {α} (goal? : Option MVarId) (t : Expr) : MetaM α := do
+  throwTacticEx `symm goal? <| MessageData.ofLazyM (es := #[t]) do
+    if let some info ← matchesPotentialRelation? t then
+      return noSymmLemmaMsg info.rel
+    else
+      return m!"Expecting a goal that is a binary relation"
+
+mutual
+
+/--
+Given `e : t`, tries applying a `@[symm]` lemma to it using forward reasoning, returning the new expression.
+-/
+private partial def applySymmFwd (goal? : Option MVarId) (e : Expr) (t tOrig : Expr) : MetaM Expr := do
+  let t ← whnfCore t
+  if !t.getAppFn.isConst then
+    throwRelError goal? tOrig
+  else if t.isAppOfArity ``Eq 3 then
+    let_expr Eq α lhs rhs := t | unreachable!
+    let us := t.getAppFn.constLevels!
+    return mkApp4 (mkConst ``Eq.symm us) α lhs rhs e
+  else if t.isAppOfArity ``HEq 4 then
+    let_expr HEq α lhs β rhs := t | unreachable!
+    let us := t.getAppFn.constLevels!
+    return mkApp5 (mkConst ``HEq.symm us) α β lhs rhs e
+  else if t.isAppOfArity ``Iff 2 then
+    let_expr Iff lhs rhs := t | unreachable!
+    return mkApp3 (mkConst ``Iff.symm []) lhs rhs e
+  else if t.isAppOfArity ``Not 1 then
+    -- Contrapose the symmetry.  If `t = ¬ (x ~ y)` then for
+    --   ¬ (x ~ y)  ->  ¬ (y ~ x)
+    -- we need
+    --   y ~ x  ->  x ~ y
+    -- To do this, we can use `applySymmBwd` and abstract the metavariable.
+    let t' := t.appArg!
+    let g1 ← mkFreshExprSyntheticOpaqueMVar t'
+    let g2 ← applySymmBwd g1.mvarId! t' t'
+    -- Abstract g2 from g1 to get implication
+    let imp ← mkLambdaFVars #[.mvar g2] g1
+    -- For safety, let's use mkAppM to validate
+    mkAppM ``mt #[imp, e]
+  else if let some { rel, .. } ← matchesRelation? t then
+    -- Search through `[symm]` keyed by the relation
+    let lems ← getSymmLemmas rel
+    if lems.isEmpty then
+      tryUnfold goal? t (throwNoSymmLemma goal? rel)
+    else
+      let mut ex? := none
+      for lem in lems do
+        try
+          return ← withNewMCtxDepth do
+            let lemE ← mkConstWithFreshMVarLevels lem
+            let (args, bis, _) ← forallMetaTelescope (← inferType lemE)
+            let some eArg := args.back? | throwError "Invalid symm lemma `{.ofConstName lem}`"
+            unless ← isDefEq eArg e do
+              let eArgTy ← instantiateMVars (← inferType eArg)
+              throwError MessageData.ofLazyM (es := #[eArgTy, t]) do
+                let (eArgTy, t) ← addPPExplicitToExposeDiff eArgTy t
+                return m!"The last hypothesis{inlineExpr eArgTy}of the symmetry lemma `{.ofConstName lem}` is not definitionally equal to{inlineExprTrailing t}"
+            synthAppInstances `symm goal? args.pop bis.pop (allowSynthFailures := false) (synthAssignedInstances := true)
+            let gs ← args.pop.filterM fun arg => not <$> arg.mvarId!.isAssigned
+            unless gs.isEmpty do
+              throwError MessageData.tagged `Tactic.unsolvedGoals <| m!"unsolved goals\n{Elab.goalsToMessageData (gs.map Expr.mvarId!).toList}"
+            instantiateMVars <| mkAppN lemE args
+        catch e =>
+          unless ex?.isSome do
+            ex? := e -- stash first failure
+      if let some e := ex? then
+        throw e
+      else
+        throwNoSymmLemma goal? rel
   else
-    throwTacticEx `symm g? <|  m!"No `[symm]` lemma registered for relation{indentExpr rel}"
-      ++ MessageData.hint' m!"Add the `[symm]` attribute to symmetry lemmas for{inlineExpr rel}to use this tactic"
+    tryUnfold goal? t (throwRelError goal? tOrig)
+where
+  tryUnfold (goal? : Option MVarId) (t : Expr) (err : MetaM Expr) : MetaM Expr := do
+    if let some t' ← withReducible <| unfoldDefinition? t then
+      applySymmFwd goal? e t' tOrig
+    else
+      err
+
+/--
+Given `goal : t`, tries applying a `@[symm]` lemma to it using backward reasoning, returning the new goal.
+-/
+private partial def applySymmBwd (goal : MVarId) (t tOrig : Expr) : MetaM MVarId := do
+  let t ← whnfCore t
+  if !t.getAppFn.isConst then
+    throwRelError goal tOrig
+  else if t.isAppOfArity ``Eq 3 then
+    let_expr Eq α lhs rhs := t | unreachable!
+    let us := t.getAppFn.constLevels!
+    let goal' ← mkFreshExprSyntheticOpaqueMVar (mkApp3 (mkConst ``Eq us) α rhs lhs)
+    goal.assign <| mkApp4 (mkConst ``Eq.symm us) α rhs lhs goal'
+    return goal'.mvarId!
+  else if t.isAppOfArity ``HEq 4 then
+    let_expr HEq α lhs β rhs := t | unreachable!
+    let us := t.getAppFn.constLevels!
+    let goal' ← mkFreshExprSyntheticOpaqueMVar (mkApp4 (mkConst ``HEq us) β rhs α lhs)
+    goal.assign <| mkApp5 (mkConst ``HEq.symm us) β α rhs lhs goal'
+    return goal'.mvarId!
+  else if t.isAppOfArity ``Iff 2 then
+    let_expr Iff lhs rhs := t | unreachable!
+    let goal' ← mkFreshExprSyntheticOpaqueMVar (mkIff rhs lhs)
+    goal.assign <| mkApp3 (mkConst ``Iff.symm []) rhs lhs goal'
+    return goal'.mvarId!
+  else if t.isAppOfArity ``Not 1 then
+    -- Contrapose the symmetry.  If `t = ¬ (x ~ y)` then we can intro `x ~ y`, apply forward
+    -- reasoning to get `y ~ x`, then revert.
+    let tag ← goal.getTag
+    let t' := t.appArg!
+    let (h, goal) ← withDefault goal.intro1
+    goal.withContext do
+      let esymm ← applySymmFwd goal (.fvar h) t' t'
+      let goal' ← mkFreshExprSyntheticOpaqueMVar (mkApp (mkConst ``Not []) (← inferType esymm))
+      goal.assign (← mkAbsurd (mkConst ``False) esymm goal')
+      let goal' := goal'.mvarId!
+      goal'.setTag tag
+      goal'.tryClear h
+  else if let some { rel, .. } ← matchesRelation? t then
+    -- Search through `[symm]` keyed by the relation
+    let lems ← getSymmLemmas rel
+    if lems.isEmpty then
+      tryUnfold goal t (throwNoSymmLemma goal rel)
+    else
+      let mut ex? := none
+      for lem in lems do
+        try
+          let (pf, t') ← withNewMCtxDepth do
+            let lemE ← mkConstWithFreshMVarLevels lem
+            let (args, bis, targetTy) ← forallMetaTelescope (← inferType lemE)
+            let some eArg := args.back? | throwError "Invalid symm lemma `{.ofConstName lem}`"
+            unless ← isDefEq targetTy t do
+              throwError MessageData.ofLazyM (es := #[targetTy, t]) do
+                let (targetTy, t) ← addPPExplicitToExposeDiff targetTy t
+                return m!"The goal{inlineExpr targetTy}of the symmetry lemma `{.ofConstName lem}` is not definitionally equal to the target{inlineExprTrailing t}"
+            synthAppInstances `symm goal args.pop bis.pop (allowSynthFailures := false) (synthAssignedInstances := true)
+            let gs ← args.pop.filterM fun arg => not <$> arg.mvarId!.isAssigned
+            unless gs.isEmpty do
+              throwError MessageData.tagged `Tactic.unsolvedGoals <| m!"unsolved goals\n{Elab.goalsToMessageData (gs.map Expr.mvarId!).toList}"
+            let pf ← instantiateMVars <| mkAppN lemE args.pop
+            let t' ← instantiateMVars <| (← inferType eArg)
+            pure (pf, t')
+          let goal' ← mkFreshExprSyntheticOpaqueMVar t' (← goal.getTag)
+          goal.assign <| mkApp pf goal'
+          return goal'.mvarId!
+        catch e =>
+          unless ex?.isSome do
+            ex? := e -- stash first failure
+      if let some e := ex? then
+        throw e
+      else
+        throwNoSymmLemma goal rel
+  else
+    tryUnfold goal t (throwRelError goal tOrig)
+where
+  tryUnfold (goal : MVarId) (t : Expr) (err : MetaM MVarId) : MetaM MVarId := do
+    if let some t' ← withReducible <| unfoldDefinition? t then
+      applySymmBwd goal t' tOrig
+    else
+      err
+
+end
 
 end Lean.Meta.Symm
 
@@ -105,13 +273,8 @@ Given a term `e : a ~ b`, constructs a term in `b ~ a` using `@[symm]` lemmas.
 The `g?` argument is used only for error reporting.
 -/
 def applySymm (g? : Option MVarId) (e : Expr) : MetaM Expr := do
-  forEachSymmLemma g? (← inferType e) fun lem tgt args body eArg => do
-    unless ← isDefEq eArg e do
-      let eArgTy ← instantiateMVars (← whnfR (← inferType eArg))
-      throwError MessageData.ofLazyM (es := #[eArgTy, tgt]) do
-        let (eArgTy, tgt) ← addPPExplicitToExposeDiff eArgTy tgt
-        return m!"The last hypothesis{indentExpr eArgTy}\nof the symmetry lemma is not definitionally equal to{indentExpr tgt}"
-    return ← mkExpectedTypeHint (mkAppN lem args) (← instantiateMVars body)
+  let t ← inferType e
+  applySymmFwd g? e t t
 
 end Lean.Expr
 
@@ -122,17 +285,10 @@ Apply a symmetry lemma (i.e. marked with `@[symm]`) to a metavariable.
 
 The type of `g` should be of the form `a ~ b`, and is used to index the symm lemmas.
 -/
-def applySymm (g : MVarId) : MetaM MVarId := do
-  forEachSymmLemma g (← g.getType) fun lem tgt args body eArg => do
-    unless ← isDefEq tgt body do
-      throwError MessageData.ofLazyM (es := #[tgt, body]) do
-        let (tgt, body) ← addPPExplicitToExposeDiff tgt body
-        return m!"The conclusion{indentExpr body}\nof the symmetry lemma is not definitionally equal to the goal{indentExpr tgt}"
-    g.assign (mkAppN lem args)
-    let g' := eArg.mvarId!
-    g'.setTag (← g.getTag)
-    g.setKind .syntheticOpaque
-    return g'
+def applySymm (g : MVarId) : MetaM MVarId :=
+  g.withContext do
+    let t ← g.getType
+    applySymmBwd g t t
 
 /-- Use a symmetry lemma (i.e. marked with `@[symm]`) to replace a hypothesis in a goal. -/
 def applySymmAt (h : FVarId) (g : MVarId) : MetaM MVarId := do
