tests/elab/relationAttrs.lean
@@ -1,0 +1,250 @@
+/-!
+# Tests of relation-related attributes
+-/
+
+set_option trace.Meta.Tactic.relation true
+set_option warn.sorry false
+
+/-!
+## @[relation] attribute
+-/
+
+/-!
+Infer lhs and rhs
+-/
+/--
+trace: [Meta.Tactic.relation] Relation `MyIff1` has 2 arguments. The first 0 argument(s) identify the relation. The lhs and rhs are argument numbers 1 and 2.
+-/
+#guard_msgs in
+@[relation]
+def MyIff1 (p q : Prop) : Prop := p ↔ q
+
+/-!
+Provide lhs and rhs
+-/
+/--
+trace: [Meta.Tactic.relation] Relation `MyIff2` has 2 arguments. The first 0 argument(s) identify the relation. The lhs and rhs are argument numbers 1 and 2.
+-/
+#guard_msgs in
+@[relation p q]
+def MyIff2 (p q : Prop) : Prop := p ↔ q
+
+/-!
+Provide lhs and rhs using indices, this time in reverse order
+-/
+/--
+trace: [Meta.Tactic.relation] Relation `MyIff3` has 2 arguments. The first 0 argument(s) identify the relation. The lhs and rhs are argument numbers 2 and 1.
+-/
+#guard_msgs in
+@[relation 2 1]
+def MyIff3 (p q : Prop) : Prop := p ↔ q
+
+/-!
+Checks that the relation hasn't already been registered
+-/
+/-- error: The relation `MyIff1` has already been registered -/
+#guard_msgs in
+attribute [relation] MyIff1
+
+/-!
+Checks that must have exactly two arguments, and they can't be same
+-/
+def MyIff4 (p q : Prop) : Prop := p ↔ q
+/-- error: Must have exactly two arguments if arguments are provided -/
+#guard_msgs in
+attribute [relation p] MyIff4
+/-- error: Must have exactly two arguments if arguments are provided -/
+#guard_msgs in
+attribute [relation p q p] MyIff4
+/-- error: Invalid argument name `p`: It has already been specified as an argument -/
+#guard_msgs in
+attribute [relation p p] MyIff4
+/--
+error: Invalid argument index `1`: The argument at this index (`p`) has already been specified as an argument
+-/
+#guard_msgs in
+attribute [relation 1 1] MyIff4
+
+/-!
+Inference fails for non-relations
+-/
+/-- error: Invalid relation: `IsZero` does not have at least two explicit arguments -/
+#guard_msgs in
+@[relation]
+def IsZero (n : Nat) : Prop := n = 0
+
+/-!
+The @[relation] attribute takes the *last* two explicit arguments by default.
+-/
+/--
+trace: [Meta.Tactic.relation] Relation `ModEq` has 3 arguments. The first 1 argument(s) identify the relation. The lhs and rhs are argument numbers 2 and 3.
+-/
+#guard_msgs in
+@[relation]
+def ModEq (n : Int) (a b : Int) : Prop := (a - b) % n == 0
+
+/-!
+## @[refl] attribute
+-/
+
+/-!
+The @[refl] attribute can auto-register relations.
+-/
+inductive MyEq1 {α : Sort _} : α → α → Prop where
+  | rfl (x : α) : MyEq1 x x
+/--
+trace: [Meta.Tactic.relation] ✅️ adding [refl] lemma `MyEq1.rfl`
+  [Meta.Tactic.relation] ✅️ Unknown relation, inferring [relation] for `MyEq1`.
+    [Meta.Tactic.relation] Relation `MyEq1` has 3 arguments. The first 1 argument(s) identify the relation. The lhs and rhs are argument numbers 2 and 3.
+-/
+#guard_msgs in
+attribute [refl] MyEq1.rfl
+
+/-!
+The @[refl] attribute also supports pre-registered relations.
+Here's a relation with reversed argumnents.
+-/
+inductive MyEq2 {α : Sort _} : α → α → Prop where
+  | rfl (x : α) : MyEq2 x x
+/--
+trace: [Meta.Tactic.relation] Relation `MyEq2` has 3 arguments. The first 1 argument(s) identify the relation. The lhs and rhs are argument numbers 3 and 2.
+-/
+#guard_msgs in
+attribute [relation 3 2] MyEq2
+/-- trace: [Meta.Tactic.relation] ✅️ adding [refl] lemma `MyEq2.rfl` -/
+#guard_msgs in
+attribute [refl] MyEq2.rfl
+
+/-!
+The @[refl] attribute checks whether the lemma proves something reflexive.
+-/
+
+theorem ModEq.symm (n a b : Int) (h : ModEq n b a) : ModEq n a b := sorry
+
+/--
+error: `[refl]` attribute only applies to lemmas concluding with `x ∼ x`, but the left-hand side
+  a
+is not definitionally equal to the right-hand side
+  b
+---
+trace: [Meta.Tactic.relation] 💥️ adding [refl] lemma `ModEq.symm`
+-/
+#guard_msgs in
+attribute [refl] ModEq.symm
+
+/-!
+The @[refl] attribute checks applicability of the lemma.
+-/
+
+/--
+error: `[refl]` lemma has unsolved goals when applied to its own conclusion
+case h
+n a : Int
+h : n > 0
+⊢ n > 0
+---
+trace: [Meta.Tactic.relation] 💥️ adding [refl] lemma `rfl_bad`
+-/
+#guard_msgs in
+@[refl]
+theorem ModEq.rfl_bad (n a : Int) (h : n > 0) : ModEq n a a := sorry
+
+
+/-!
+## @[symm] attribute
+-/
+
+/-!
+Validates that the conclusion is a constant application
+-/
+/--
+error: `[symm]` attribute only applies to lemmas proving `x ∼ y → y ~ x`, where the relation is a constant application, but the relation is not a constant application: `Type`
+---
+trace: [Meta.Tactic.relation] 💥️ adding [symm] lemma `symm_bad1`
+-/
+#guard_msgs in
+@[symm] def symm_bad1 : Type := Nat
+
+/-!
+The @[symm] attribute can auto-register relations.
+-/
+inductive MyEq3 {α : Sort _} : α → α → Prop where
+  | rfl (x : α) : MyEq3 x x
+def MyEq3.symm {α} (x y : α) : MyEq3 x y → MyEq3 y x
+  | .rfl _ => .rfl _
+/--
+trace: [Meta.Tactic.relation] ✅️ adding [symm] lemma `MyEq3.symm`
+  [Meta.Tactic.relation] ✅️ Unknown relation, inferring [relation] for `MyEq3`.
+    [Meta.Tactic.relation] Relation `MyEq3` has 3 arguments. The first 1 argument(s) identify the relation. The lhs and rhs are argument numbers 2 and 3.
+-/
+#guard_msgs in
+attribute [symm] MyEq3.symm
+
+/-!
+The @[refl] attribute also supports pre-registered relations.
+Here's a relation with reversed argumnents.
+-/
+inductive MyEq4 {α : Sort _} : α → α → Prop where
+  | rfl (x : α) : MyEq4 x x
+def MyEq4.symm {α} (x y : α) : MyEq4 x y → MyEq4 y x
+  | .rfl _ => .rfl _
+/--
+trace: [Meta.Tactic.relation] Relation `MyEq4` has 3 arguments. The first 1 argument(s) identify the relation. The lhs and rhs are argument numbers 3 and 2.
+-/
+#guard_msgs in
+attribute [relation 3 2] MyEq4
+/-- trace: [Meta.Tactic.relation] ✅️ adding [symm] lemma `MyEq4.symm` -/
+#guard_msgs in
+attribute [symm] MyEq4.symm
+
+/-!
+The @[symm] attribute checks whether the lemma proves something symmetric-like.
+-/
+
+/-- trace: [Meta.Tactic.relation] ✅️ adding [symm] lemma `ModEq.symm` -/
+#guard_msgs in attribute [symm] ModEq.symm
+
+/--
+error: `[symm]` attribute only applies to lemmas proving `x ~ y → y ∼ x`, but the conclusion's left-hand side
+  a
+is not definitionally equal to the hypothesis's right-hand side
+  b
+---
+trace: [Meta.Tactic.relation] 💥️ adding [symm] lemma `symm_bad`
+-/
+#guard_msgs in @[symm] theorem ModEq.symm_bad (n a b : Int) (h : ModEq n a b) : ModEq n a b := sorry
+
+/--
+error: `[symm]` attribute only applies to lemmas proving `x ~ y → y ∼ x`, but the conclusion's right-hand side
+  b
+is not definitionally equal to the hypothesis's left-hand side
+  a
+---
+trace: [Meta.Tactic.relation] 💥️ adding [symm] lemma `symm_bad'`
+-/
+#guard_msgs in @[symm] theorem ModEq.symm_bad' (n a b : Int) (h : ModEq n a a) : ModEq n a b := sorry
+
+/-!
+The @[symm] attribute doesn't check that the lemma is morally symmetric.
+-/
+
+/-- trace: [Meta.Tactic.relation] ✅️ adding [symm] lemma `symm_questionable` -/
+#guard_msgs in @[symm] theorem ModEq.symm_questionable (n a : Int) (h : ModEq n a a) : ModEq n a a := sorry
+
+/-!
+The @[symm] attribute checks applicability of the lemma.
+-/
+
+/--
+error: `[symm]` lemma has unsolved goals when applied to its own conclusion
+case h
+n a b : Int
+h : n > 0
+h' : ModEq n b a
+⊢ n > 0
+---
+trace: [Meta.Tactic.relation] 💥️ adding [symm] lemma `symm_bad2`
+-/
+#guard_msgs in
+@[symm]
+theorem ModEq.symm_bad2 (n a b : Int) (h : n > 0) (h' : ModEq n b a) : ModEq n a b := sorry
